rename files

doc/tutorial/code/solutions_universes/Ex10a.fst
@@ -1,6 +1,6 @@
 module Ex10a
 
-open FStar.List
+open FStar.List.Tot
 open FStar.Heap
 
 type file = string
@@ -12,13 +12,19 @@ type entry =
 type db = list entry
 
 let canWrite db file =
-  is_Some (find (function Writable x -> x=file | _ -> false) db)
+  is_Some (tryFind (function Writable x -> x=file | _ -> false) db)
+
 
 let canRead db file =
-  is_Some (find (function Readable x | Writable x -> x=file) db)
+  is_Some (tryFind (function Readable x | Writable x -> x=file) db)
+
 
 assume val acls: ref db
-type canRead_t f h  = canRead  (sel h acls) f == true
+
+
+type canRead_t f h  = canRead  (sel h acls) f  == true
+
+
 type canWrite_t f h = canWrite (sel h acls) f == true
 
 
@@ -27,32 +33,41 @@ val grant : e:entry -> ST unit (requires (fun h -> True))
 let grant e = ST.write acls (e::ST.read acls)
 
 val revoke: e:entry -> ST unit (requires (fun h -> True))
-                               (ensures (fun h x h' -> not(List.mem e (sel h' acls))))
+                               (ensures (fun h x h' -> not(mem e (sel h' acls))))
 let revoke e =
-  let db = filterT (fun e' -> e<>e') (ST.read acls) in
+  let db = filter (fun e' -> e<>e') (ST.read acls) in
   ST.write acls db
+
 
 (* two dangerous primitives *)
 assume val read:   file:string -> ST string
-                                     (requires (CanRead file))
-                                     (ensures (fun h s h' -> h=h'))
+                                     (requires (canRead_t file))
+                                     (ensures (fun h s h' -> modifies_none h h'))
+
 
 assume val delete: file:string -> ST unit
-                                     (requires (CanWrite file))
-                                     (ensures (fun h s h' -> h=h'))
+                                     (requires (canWrite_t file))
+                                     (ensures (fun h s h' -> modifies_none h h'))
 
-val safe_delete: file -> All unit (fun h -> True) (fun h x h' -> h==h')
+
+val safe_delete: file -> All unit 
+			    (requires (fun h -> True))
+			    (ensures (fun h x h' -> modifies_none h h'))
+
+
 let safe_delete file =
   if canWrite !acls file
   then delete file
-  else failwith "unwritable"
+  else  
+  failwith "unwritable"
+
 
 val test_acls: file -> unit
 let test_acls f =
   grant (Readable f);     (* ok *)
   let _ = read f in       (* ok --- it's in the acl *)
-  (* delete f;               (\* not ok --- we're only allowed to read it *\) *)
+  //delete f;               (* not ok --- we're only allowed to read it *) 
   safe_delete f;          (* ok, but fails dynamically *)
   revoke (Readable f);
-  (* let _ = read f in       (\* not ok any more *\) *)
+  //let _ = read f in       (* not ok any more *) 
   ()
